Use uint16_t

code/frodo/Hacl.Impl.PQ.Lib.fst
@@ -9,140 +9,135 @@ open FStar.Mul
 open FStar.Math.Lemmas
 
 inline_for_extraction
-type numeric_t = inttype
+type numeric_t = uint16
 
 inline_for_extraction
 let lbytes len = lbuffer uint8 len
 
 inline_for_extraction
+noextract
 let v = size_v
 
 inline_for_extraction
-val numeric:
-  #t:inttype -> x:nat{x <= maxint t} -> uint_t t
-let numeric #t x =
-  match t with
-  | U8 -> u8 x
-  | U16 -> u16 x
-  | U32 -> u32 x
-  | U64 -> u64 x
-  | U128 -> u128 x
-  | SIZE -> size x
-  | NATm m -> modulo x m
-
-inline_for_extraction
-val to_numeric:
-  #t:inttype -> t1:inttype -> x:uint_t t -> r:uint_t t1{uint_v r == uint_v x % modulus t1}
-let to_numeric #t t1 x =
-  match t, t1 with
-  | U16, U16 -> x
-  | U16, NATm m -> modulo ((Lib.RawIntTypes.uint_to_nat x) % m) m
-  | NATm m, U16 -> u16 ((Lib.RawIntTypes.uint_to_nat x) % modulus U16)
-  | _ -> admit()
-
-inline_for_extraction
-val matrix_t:
-  t:numeric_t -> n1:size_t -> n2:size_t -> Type0
-let matrix_t t n1 n2 = lbuffer (uint_t t) (v (n1 *. n2))
+val matrix_t: n1:size_t -> n2:size_t -> Type0
+let matrix_t n1 n2 = lbuffer uint16 (v (n1 *. n2))
 
 val matrix_create:
-  t:numeric_t -> n1:size_t -> n2:size_t ->
-  StackInline (matrix_t t n1 n2)
+  n1:size_t -> n2:size_t ->
+  StackInline (matrix_t n1 n2)
   (requires (fun h -> True))
-  (ensures (fun h0 r h1 -> True))
+  (ensures (fun h0 r h1 -> live h1 r))
   [@ "substitute"]
-let matrix_create t n1 n2 =
-  create (n1 *. n2) (numeric #t 0)
+let matrix_create n1 n2 =
+  create #uint16 (n1 *. n2) (u16 0)
 
 val mget:
-  #t:numeric_t -> n1:size_t -> n2:size_t ->
-  a:matrix_t t n1 n2 ->
-  i:size_t{v i < v n1} -> j:size_t{v j < v n2} -> Stack (uint_t t)
+  #n1:size_t -> #n2:size_t ->
+  a:matrix_t n1 n2 ->
+  i:size_t{v i < v n1} -> j:size_t{v j < v n2} -> Stack uint16
   (requires (fun h -> live h a))
   (ensures (fun h0 r h1 -> True))
   [@ "substitute"]
-let mget #t n1 n2 a i j =
+let mget #n1 #n2 a i j =
   assume (v (i *. n2 +. j) < v (n1 *. n2));
   a.(i *. n2 +. j)
 
 val mset:
-  #t:numeric_t -> n1:size_t -> n2:size_t ->
-  a:matrix_t t n1 n2 ->
+  #n1:size_t -> #n2:size_t ->
+  a:matrix_t n1 n2 ->
   i:size_t{v i < v n1} -> j:size_t{v j < v n2} ->
-  vij:uint_t t -> Stack unit
+  vij:uint16 -> Stack unit
   (requires (fun h -> live h a))
   (ensures (fun h0 r h1 -> True))
   [@ "substitute"]
-let mset #t n1 n2 a i j vij =
+let mset #n1 #n2 a i j vij =
   assume (v (i *. n2 +. j) < v (n1 *. n2));
   a.(i *. n2 +. j) <- vij
 
 //modifies a
 val matrix_add:
-  #t:numeric_t -> n1:size_t -> n2:size_t ->
-  a:matrix_t t n1 n2 -> b:matrix_t t n1 n2 ->
+  #n1:size_t -> #n2:size_t ->
+  a:matrix_t n1 n2 -> b:matrix_t n1 n2 ->
   Stack unit
   (requires (fun h -> True))
   (ensures (fun h0 r h1 -> True))
   [@"c_inline"]
-let matrix_add #t n1 n2 a b =
+let matrix_add #n1 #n2 a b =
   admit();
   let h0 = FStar.HyperStack.ST.get () in
   loop_nospec #h0 n1 a
   (fun i ->
     loop_nospec #h0 n2 a
     (fun j ->
-      let aij = mget n1 n2 a i j in
-      let bij = mget n1 n2 b i j in
+      let aij = mget a i j in
+      let bij = mget b i j in
       let res = add_mod aij bij in
-      mset n1 n2 a i j res
+      mset a i j res
     )
   )
 
 //modifies a
 val matrix_sub:
-  #t:numeric_t -> n1:size_t -> n2:size_t ->
-  a:matrix_t t n1 n2 -> b:matrix_t t n1 n2 ->
+  #n1:size_t -> #n2:size_t ->
+  a:matrix_t n1 n2 -> b:matrix_t n1 n2 ->
   Stack unit
   (requires (fun h -> True))
   (ensures (fun h0 r h1 -> True))
   [@"c_inline"]
-let matrix_sub #t n1 n2 a b =
+let matrix_sub #n1 #n2 a b =
   admit();
   let h0 = FStar.HyperStack.ST.get () in
   loop_nospec #h0 n1 a
   (fun i ->
     loop_nospec #h0 n2 a
     (fun j ->
-      let aij = mget n1 n2 a i j in
-      let bij = mget n1 n2 b i j in
+      let aij = mget a i j in
+      let bij = mget b i j in
       let res = sub_mod aij bij in
-      mset n1 n2 a i j res
+      mset a i j res
     )
   )
 
 val matrix_mul:
-  #t:numeric_t -> n1:size_t -> n2:size_t -> n3:size_t ->
-  a:matrix_t t n1 n2 -> b:matrix_t t n2 n3 ->
-  c:matrix_t t n1 n3 -> Stack unit
+  #n1:size_t -> #n2:size_t -> #n3:size_t ->
+  a:matrix_t n1 n2 -> b:matrix_t n2 n3 ->
+  c:matrix_t n1 n3 -> Stack unit
   (requires (fun h -> True))
   (ensures (fun h0 r h1 -> True))
   [@"c_inline"]
-let matrix_mul #t n1 n2 n3 a b c =
+let matrix_mul #n1 #n2 #n3 a b c =
   admit();
   let h0 = FStar.HyperStack.ST.get () in
   loop_nospec #h0 n1 c
   (fun i ->
     loop_nospec #h0 n3 c
     (fun k ->
-      mset n1 n3 c i k (numeric #t 0);
+      mset c i k (u16 0);
       loop_nospec #h0 n2 c
       (fun j ->
-	let aij = mget n1 n2 a i j in
-	let bjk = mget n2 n3 b j k in
-	let cik = mget n1 n3 c i k in
+	let aij = mget a i j in
+	let bjk = mget b j k in
+	let cik = mget c i k in
 	let res = cik +. aij *. bjk in
-	mset n1 n3 c i k res
+	mset c i k res
       )
     )
   )
+
+
+val main: unit -> St unit
+let main _ =
+  push_frame();
+  let m1 = matrix_create (size 2) (size 2) in
+  let m2 = matrix_create (size 2) (size 2) in
+  admit();
+  mset m1 (size 0) (size 0) (u16 0);
+  mset m1 (size 0) (size 1) (u16 1);
+  mset m1 (size 1) (size 0) (u16 2);
+  mset m1 (size 1) (size 1) (u16 3);
+  mset m2 (size 0) (size 0) (u16 0);
+  mset m2 (size 0) (size 1) (u16 1);
+  mset m2 (size 1) (size 0) (u16 2);
+  mset m2 (size 1) (size 1) (u16 3);
+  matrix_add m1 m2;
+  pop_frame()
